spec/design/ARM_HYP/ArchHypervisor_H.thy
@@ -1,3 +1,5 @@
+(* THIS FILE WAS AUTOMATICALLY GENERATED. DO NOT EDIT. *)
+(* instead, see the skeleton file ArchHypervisor_H.thy *)
 (*
  * Copyright 2014, General Dynamics C4 Systems
  *
@@ -15,18 +17,66 @@
 theory ArchHypervisor_H
 imports
   "../CNode_H"
+  "../FaultHandlerDecls_H"
 (*  "../KI_Decls_H"
   ArchVSpaceDecls_H *)
 begin
 context Arch begin global_naming ARM_HYP_H
 
-
 consts'
-handleHypervisorFault :: "machine_word \<Rightarrow> hyp_fault_type \<Rightarrow> unit kernel"
+countTrailingZeros :: "('b :: {HS_bit, finiteBit}) \<Rightarrow> nat"
+
+defs countTrailingZeros_def:
+"countTrailingZeros w \<equiv>
+    length \<circ> takeWhile Not \<circ> map (testBit w) $ [0  .e.  finiteBitSize w - 1]"
 
 
-defs handleHypervisorFault_def:
-"handleHypervisorFault arg1 hyp \<equiv> case hyp of ARMNoHypFaults \<Rightarrow> haskell_fail []"
+definition
+virqSetEOIIRQEN :: "virq \<Rightarrow> machine_word \<Rightarrow> virq"
+where
+"virqSetEOIIRQEN virq v \<equiv>
+    (virq && complement 0x80000) || ((v `~shiftL~` 19) && 0x80000)"
+
+definition
+vgicMaintenance :: "unit kernel"
+where
+"vgicMaintenance \<equiv>
+    let
+        irqIndex = (\<lambda>  eisr0 eisr1.
+            if eisr0 \<noteq> 0 then countTrailingZeros eisr0
+                          else countTrailingZeros eisr1);
+        badIndex = (\<lambda>  irq_idx. doMachineOp $ ((do
+              virq \<leftarrow> get_gic_vcpu_ctrl_lr (fromIntegral irq_idx);
+              set_gic_vcpu_ctrl_lr (fromIntegral irq_idx) $ virqSetEOIIRQEN virq 0
+        od)
+              ))
+    in
+                         (do
+    ct \<leftarrow> gets ksCurThread;
+    runnable \<leftarrow> isRunnable ct;
+    when runnable $ (do
+      eisr0 \<leftarrow> doMachineOp $ get_gic_vcpu_ctrl_eisr0;
+      eisr1 \<leftarrow> doMachineOp $ get_gic_vcpu_ctrl_eisr1;
+      flags \<leftarrow> doMachineOp $ get_gic_vcpu_ctrl_misr;
+      vgic_misr_eoi \<leftarrow> return ( 1);
+      fault \<leftarrow>
+          if (flags && vgic_misr_eoi \<noteq> 0)
+          then
+              if (eisr0 = 0 \<and> eisr1 = 0)
+                  then return $ VGICMaintenance [0, 0]
+                  else ((do
+                      irq_idx \<leftarrow> return ( irqIndex eisr0 eisr1);
+                      gic_vcpu_num_list_regs \<leftarrow>
+                          gets (armKSGICVCPUNumListRegs \<circ> ksArchState);
+                      when (irq_idx < gic_vcpu_num_list_regs) (badIndex irq_idx);
+                      return $ VGICMaintenance [fromIntegral irq_idx, 1]
+                  od)
+                      )
+          else return $ VGICMaintenance [0, 0];
+      ct \<leftarrow> getCurThread;
+      handleFault ct $ ArchFault fault
+    od)
+                         od)"
 
 definition
 vcpuEnable :: "machine_word \<Rightarrow> unit kernel"
@@ -34,7 +84,7 @@ where
 "vcpuEnable vcpuPtr\<equiv> (do
     vcpu \<leftarrow> getObject vcpuPtr;
     doMachineOp $ (do
-        setSCTLR (vcpuSCTLR vcpu);
+        setSCTLR (vcpuRegs vcpu VCPURegSCTLR);
         setHCR hcrVCPU;
         isb;
         set_gic_vcpu_ctrl_hcr (vgicHCR \<circ> vcpuVGIC $ vcpu)
@@ -51,9 +101,10 @@ where
            vcpu \<leftarrow> getObject vcpuPtr;
            hcr \<leftarrow> doMachineOp get_gic_vcpu_ctrl_hcr;
            sctlr \<leftarrow> doMachineOp getSCTLR;
+           regs' \<leftarrow> return ( vcpuRegs vcpu  aLU  [(VCPURegSCTLR, sctlr)]);
            setObject vcpuPtr $ vcpu \<lparr>
-                 vcpuSCTLR := sctlr
-               , vcpuVGIC := (vcpuVGIC vcpu) \<lparr> vgicHCR := hcr \<rparr>
+                 vcpuVGIC := (vcpuVGIC vcpu) \<lparr> vgicHCR := hcr \<rparr>
+               , vcpuRegs := regs'
                \<rparr>
           od)
         | None \<Rightarrow>   return ()
@@ -85,16 +136,48 @@ where
     vmcr \<leftarrow> doMachineOp get_gic_vcpu_ctrl_vmcr;
     apr \<leftarrow> doMachineOp get_gic_vcpu_ctrl_apr;
     numListRegs \<leftarrow> gets (armKSGICVCPUNumListRegs \<circ> ksArchState);
-    gicIndices \<leftarrow> return ( [0 .e. numListRegs- 1]);
-    lrVals \<leftarrow> doMachineOp $ mapM get_gic_vcpu_ctrl_lr gicIndices;
+    gicIndices \<leftarrow> return ( init [0 .e. numListRegs]);
+    lrVals \<leftarrow> doMachineOp $ mapM (get_gic_vcpu_ctrl_lr \<circ> fromIntegral) gicIndices;
     vcpuLR \<leftarrow> return ( (vgicLR \<circ> vcpuVGIC $ vcpu)  aLU  zip gicIndices lrVals);
+    lr_svc \<leftarrow> doMachineOp get_lr_svc;
+    sp_svc \<leftarrow> doMachineOp get_sp_svc;
+    lr_abt \<leftarrow> doMachineOp get_lr_abt;
+    sp_abt \<leftarrow> doMachineOp get_sp_abt;
+    lr_und \<leftarrow> doMachineOp get_lr_und;
+    sp_und \<leftarrow> doMachineOp get_sp_und;
+    lr_irq \<leftarrow> doMachineOp get_lr_irq;
+    sp_irq \<leftarrow> doMachineOp get_sp_irq;
+    lr_fiq \<leftarrow> doMachineOp get_lr_fiq;
+    sp_fiq \<leftarrow> doMachineOp get_sp_fiq;
+    r8_fiq \<leftarrow> doMachineOp get_r8_fiq;
+    r9_fiq \<leftarrow> doMachineOp get_r9_fiq;
+    r10_fiq \<leftarrow> doMachineOp get_r10_fiq;
+    r11_fiq \<leftarrow> doMachineOp get_r11_fiq;
+    r12_fiq \<leftarrow> doMachineOp get_r12_fiq;
+    regs' \<leftarrow> return ( (vcpuRegs vcpu)  aLU  [(VCPURegSCTLR, sctlr)
+                                   ,(VCPURegLRsvc, lr_svc)
+                                   ,(VCPURegSPsvc, sp_svc)
+                                   ,(VCPURegLRabt, lr_abt)
+                                   ,(VCPURegSPabt, sp_abt)
+                                   ,(VCPURegLRund, lr_und)
+                                   ,(VCPURegSPund, sp_und)
+                                   ,(VCPURegLRirq, lr_irq)
+                                   ,(VCPURegSPirq, sp_irq)
+                                   ,(VCPURegLRfiq, lr_fiq)
+                                   ,(VCPURegSPfiq, sp_fiq)
+                                   ,(VCPURegR8fiq, r8_fiq)
+                                   ,(VCPURegR9fiq, r9_fiq)
+                                   ,(VCPURegR10fiq, r10_fiq)
+                                   ,(VCPURegR11fiq, r11_fiq)
+                                   ,(VCPURegR12fiq, r12_fiq)
+                                   ]);
     setObject vcpuPtr $ vcpu \<lparr>
-          vcpuSCTLR := sctlr
-        , vcpuACTLR := actlr
+          vcpuACTLR := actlr
         , vcpuVGIC := (vcpuVGIC vcpu) \<lparr> vgicHCR := hcr
                                      , vgicVMCR := vmcr
                                      , vgicAPR := apr
                                      , vgicLR := vcpuLR \<rparr>
+        , vcpuRegs := regs'
         \<rparr>;
     doMachineOp isb
     od)
@@ -112,7 +195,22 @@ where
     doMachineOp $ (do
         set_gic_vcpu_ctrl_vmcr (vgicVMCR vgic);
         set_gic_vcpu_ctrl_apr (vgicAPR vgic);
-        mapM_x (uncurry set_gic_vcpu_ctrl_lr) (map (\<lambda> i. (i, (vgicLR vgic) i)) [0 .e. gicVCPUMaxNumLR- 1]);
+        mapM_x (uncurry set_gic_vcpu_ctrl_lr) (map (\<lambda> i. (fromIntegral i, (vgicLR vgic) i)) [0 .e. gicVCPUMaxNumLR- 1]);
+        set_lr_svc (vcpuRegs vcpu VCPURegLRsvc);
+        set_sp_svc (vcpuRegs vcpu VCPURegSPsvc);
+        set_lr_abt (vcpuRegs vcpu VCPURegLRabt);
+        set_sp_abt (vcpuRegs vcpu VCPURegSPabt);
+        set_lr_und (vcpuRegs vcpu VCPURegLRund);
+        set_sp_und (vcpuRegs vcpu VCPURegSPund);
+        set_lr_irq (vcpuRegs vcpu VCPURegLRirq);
+        set_sp_irq (vcpuRegs vcpu VCPURegSPirq);
+        set_lr_fiq (vcpuRegs vcpu VCPURegLRfiq);
+        set_sp_fiq (vcpuRegs vcpu VCPURegSPfiq);
+        set_r8_fiq (vcpuRegs vcpu VCPURegR8fiq);
+        set_r9_fiq (vcpuRegs vcpu VCPURegR9fiq);
+        set_r10_fiq (vcpuRegs vcpu VCPURegR10fiq);
+        set_r11_fiq (vcpuRegs vcpu VCPURegR11fiq);
+        set_r12_fiq (vcpuRegs vcpu VCPURegR12fiq);
         setACTLR (vcpuACTLR vcpu)
     od);
     vcpuEnable vcpuPtr
@@ -124,19 +222,10 @@ where
 "vcpuInvalidateActive\<equiv> (do
     hsCurVCPU \<leftarrow> gets (armHSCurVCPU \<circ> ksArchState);
     (case hsCurVCPU of
-          Some (vcpuPtr, True) \<Rightarrow>   (do
-            vcpuDisable Nothing;
-            modifyArchState (\<lambda> s. s \<lparr> armHSCurVCPU := Just (vcpuPtr, False) \<rparr>)
-          od)
+          Some (vcpuPtr, True) \<Rightarrow>   vcpuDisable Nothing
         | _ \<Rightarrow>   return ()
-        )
-od)"
-
-definition
-"vcpuCleanInvalidateActive\<equiv> (do
-    hsCurVCPU \<leftarrow> gets (armHSCurVCPU \<circ> ksArchState);
-    vcpuSave hsCurVCPU;
-    vcpuInvalidateActive
+        );
+    modifyArchState (\<lambda> s. s \<lparr> armHSCurVCPU := Nothing \<rparr>)
 od)"
 
 definition
@@ -174,7 +263,7 @@ where
                     when (Not active) $ (do
                         doMachineOp isb;
                         vcpuEnable new;
-                        modifyArchState (\<lambda> s. s \<lparr> armHSCurVCPU := Just (new, False) \<rparr>)
+                        modifyArchState (\<lambda> s. s \<lparr> armHSCurVCPU := Just (new, True) \<rparr>)
                     od)
                 )
         )
@@ -182,6 +271,16 @@ where
   od)
   )"
 
+
+consts'
+handleHypervisorFault :: "machine_word \<Rightarrow> hyp_fault_type \<Rightarrow> unit kernel"
+
+defs handleHypervisorFault_def:
+"handleHypervisorFault thread x1\<equiv> (case x1 of
+    (ARMVCPUFault hsr) \<Rightarrow>    (
+    handleFault thread (ArchFault $ VCPUFault $ fromIntegral hsr)
+    )
+  )"
 
 
 end
