spec/design/ARM_HYP/ArchInterrupt_H.thy
@@ -1,3 +1,5 @@
+(* THIS FILE WAS AUTOMATICALLY GENERATED. DO NOT EDIT. *)
+(* instead, see the skeleton file ArchInterrupt_H.thy *)
 (*
  * Copyright 2014, General Dynamics C4 Systems
  *
@@ -11,7 +13,7 @@
 theory ArchInterrupt_H
 imports "../RetypeDecls_H" "../CNode_H" "../InterruptDecls_H" ArchInterruptDecls_H
 begin
-context Arch begin global_naming ARM_H
+context Arch begin global_naming ARM_HYP_H
 
 defs decodeIRQControlInvocation_def:
 "decodeIRQControlInvocation arg1 arg2 arg3 arg4 \<equiv> throw IllegalOperation"
@@ -22,6 +24,18 @@ defs performIRQControl_def:
 defs checkIRQ_def:
 "checkIRQ irq\<equiv> rangeCheck irq (fromEnum minIRQ) (fromEnum maxIRQ)"
 
+defs handleReservedIRQ_def:
+"handleReservedIRQ irq\<equiv> (do
+    when (fromEnum irq = fromEnum irqVGICMaintenance) vgicMaintenance;
+    return ()
+od)"
+
+
+definition initInterruptController :: "unit kernel"
+  where "initInterruptController \<equiv> (do
+    setIRQState IRQReserved $ irqVGICMaintenance;
+    return ()
+od)"
 
 end
 end
