spec/design/ARM_HYP/ArchStateData_H.thy
@@ -1,3 +1,5 @@
+(* THIS FILE WAS AUTOMATICALLY GENERATED. DO NOT EDIT. *)
+(* instead, see the skeleton file ArchStateData_H.thy *)
 (*
  * Copyright 2014, General Dynamics C4 Systems
  *
@@ -20,30 +22,10 @@ imports
   ArchTypes_H
   ArchStructures_H
 begin
-context Arch begin global_naming ARM_H
+context Arch begin global_naming ARM_HYP_H
 
 datatype kernel_state =
-    ARMKernelState machine_word "asid \<Rightarrow> ((machine_word) option)" "hardware_asid \<Rightarrow> (asid option)" hardware_asid "asid \<Rightarrow> ((hardware_asid * machine_word) option)" machine_word "(machine_word * bool) option" nat "machine_word \<Rightarrow> arm_vspace_region_use"
-
-primrec
-  armKSGlobalsFrame :: "kernel_state \<Rightarrow> machine_word"
-where
-  "armKSGlobalsFrame (ARMKernelState v0 v1 v2 v3 v4 v5 v6 v7) = v0"
-
-primrec
-  armKSASIDTable :: "kernel_state \<Rightarrow> asid \<Rightarrow> ((machine_word) option)"
-where
-  "armKSASIDTable (ARMKernelState v0 v1 v2 v3 v4 v5 v6 v7) = v1"
-
-primrec
-  armKSGlobalPD :: "kernel_state \<Rightarrow> machine_word"
-where
-  "armKSGlobalPD (ARMKernelState v0 v1 v2 v3 v4 v5 v6 v7) = v5"
-
-primrec
-  armKSHWASIDTable :: "kernel_state \<Rightarrow> hardware_asid \<Rightarrow> (asid option)"
-where
-  "armKSHWASIDTable (ARMKernelState v0 v1 v2 v3 v4 v5 v6 v7) = v2"
+    ARMKernelState "asid \<Rightarrow> ((machine_word) option)" "hardware_asid \<Rightarrow> (asid option)" hardware_asid "asid \<Rightarrow> ((hardware_asid * machine_word) option)" "(machine_word * bool) option" nat machine_word "machine_word \<Rightarrow> arm_vspace_region_use"
 
 primrec
   armKSKernelVSpace :: "kernel_state \<Rightarrow> machine_word \<Rightarrow> arm_vspace_region_use"
@@ -51,39 +33,39 @@ where
   "armKSKernelVSpace (ARMKernelState v0 v1 v2 v3 v4 v5 v6 v7) = v7"
 
 primrec
+  armKSASIDTable :: "kernel_state \<Rightarrow> asid \<Rightarrow> ((machine_word) option)"
+where
+  "armKSASIDTable (ARMKernelState v0 v1 v2 v3 v4 v5 v6 v7) = v0"
+
+primrec
+  armKSGICVCPUNumListRegs :: "kernel_state \<Rightarrow> nat"
+where
+  "armKSGICVCPUNumListRegs (ARMKernelState v0 v1 v2 v3 v4 v5 v6 v7) = v5"
+
+primrec
+  armKSHWASIDTable :: "kernel_state \<Rightarrow> hardware_asid \<Rightarrow> (asid option)"
+where
+  "armKSHWASIDTable (ARMKernelState v0 v1 v2 v3 v4 v5 v6 v7) = v1"
+
+primrec
   armHSCurVCPU :: "kernel_state \<Rightarrow> (machine_word * bool) option"
 where
-  "armHSCurVCPU (ARMKernelState v0 v1 v2 v3 v4 v5 v6 v7 v8) = v6"
+  "armHSCurVCPU (ARMKernelState v0 v1 v2 v3 v4 v5 v6 v7) = v4"
+
+primrec
+  armUSGlobalPD :: "kernel_state \<Rightarrow> machine_word"
+where
+  "armUSGlobalPD (ARMKernelState v0 v1 v2 v3 v4 v5 v6 v7) = v6"
 
 primrec
   armKSNextASID :: "kernel_state \<Rightarrow> hardware_asid"
 where
-  "armKSNextASID (ARMKernelState v0 v1 v2 v3 v4 v5 v6 v7) = v3"
+  "armKSNextASID (ARMKernelState v0 v1 v2 v3 v4 v5 v6 v7) = v2"
 
 primrec
   armKSASIDMap :: "kernel_state \<Rightarrow> asid \<Rightarrow> ((hardware_asid * machine_word) option)"
 where
-  "armKSASIDMap (ARMKernelState v0 v1 v2 v3 v4 v5 v6 v7) = v4"
-
-primrec
-  armKSGlobalsFrame_update :: "(machine_word \<Rightarrow> machine_word) \<Rightarrow> kernel_state \<Rightarrow> kernel_state"
-where
-  "armKSGlobalsFrame_update f (ARMKernelState v0 v1 v2 v3 v4 v5 v6 v7) = ARMKernelState (f v0) v1 v2 v3 v4 v5 v6 v7"
-
-primrec
-  armKSASIDTable_update :: "((asid \<Rightarrow> ((machine_word) option)) \<Rightarrow> (asid \<Rightarrow> ((machine_word) option))) \<Rightarrow> kernel_state \<Rightarrow> kernel_state"
-where
-  "armKSASIDTable_update f (ARMKernelState v0 v1 v2 v3 v4 v5 v6 v7) = ARMKernelState v0 (f v1) v2 v3 v4 v5 v6 v7"
-
-primrec
-  armKSGlobalPD_update :: "(machine_word \<Rightarrow> machine_word) \<Rightarrow> kernel_state \<Rightarrow> kernel_state"
-where
-  "armKSGlobalPD_update f (ARMKernelState v0 v1 v2 v3 v4 v5 v6 v7) = ARMKernelState v0 v1 v2 v3 v4 (f v5) v6 v7"
-
-primrec
-  armKSHWASIDTable_update :: "((hardware_asid \<Rightarrow> (asid option)) \<Rightarrow> (hardware_asid \<Rightarrow> (asid option))) \<Rightarrow> kernel_state \<Rightarrow> kernel_state"
-where
-  "armKSHWASIDTable_update f (ARMKernelState v0 v1 v2 v3 v4 v5 v6 v7) = ARMKernelState v0 v1 (f v2) v3 v4 v5 v6 v7"
+  "armKSASIDMap (ARMKernelState v0 v1 v2 v3 v4 v5 v6 v7) = v3"
 
 primrec
   armKSKernelVSpace_update :: "((machine_word \<Rightarrow> arm_vspace_region_use) \<Rightarrow> (machine_word \<Rightarrow> arm_vspace_region_use)) \<Rightarrow> kernel_state \<Rightarrow> kernel_state"
@@ -91,197 +73,67 @@ where
   "armKSKernelVSpace_update f (ARMKernelState v0 v1 v2 v3 v4 v5 v6 v7) = ARMKernelState v0 v1 v2 v3 v4 v5 v6 (f v7)"
 
 primrec
+  armKSASIDTable_update :: "((asid \<Rightarrow> ((machine_word) option)) \<Rightarrow> (asid \<Rightarrow> ((machine_word) option))) \<Rightarrow> kernel_state \<Rightarrow> kernel_state"
+where
+  "armKSASIDTable_update f (ARMKernelState v0 v1 v2 v3 v4 v5 v6 v7) = ARMKernelState (f v0) v1 v2 v3 v4 v5 v6 v7"
+
+primrec
+  armKSGICVCPUNumListRegs_update :: "(nat \<Rightarrow> nat) \<Rightarrow> kernel_state \<Rightarrow> kernel_state"
+where
+  "armKSGICVCPUNumListRegs_update f (ARMKernelState v0 v1 v2 v3 v4 v5 v6 v7) = ARMKernelState v0 v1 v2 v3 v4 (f v5) v6 v7"
+
+primrec
+  armKSHWASIDTable_update :: "((hardware_asid \<Rightarrow> (asid option)) \<Rightarrow> (hardware_asid \<Rightarrow> (asid option))) \<Rightarrow> kernel_state \<Rightarrow> kernel_state"
+where
+  "armKSHWASIDTable_update f (ARMKernelState v0 v1 v2 v3 v4 v5 v6 v7) = ARMKernelState v0 (f v1) v2 v3 v4 v5 v6 v7"
+
+primrec
   armHSCurVCPU_update :: "(((machine_word * bool) option) \<Rightarrow> ((machine_word * bool) option)) \<Rightarrow> kernel_state \<Rightarrow> kernel_state"
 where
-  "armHSCurVCPU_update f (ARMKernelState v0 v1 v2 v3 v4 v5 v6 v7 v8) = ARMKernelState v0 v1 v2 v3 v4 v5 (f v6) v7 v8"
+  "armHSCurVCPU_update f (ARMKernelState v0 v1 v2 v3 v4 v5 v6 v7) = ARMKernelState v0 v1 v2 v3 (f v4) v5 v6 v7"
+
+primrec
+  armUSGlobalPD_update :: "(machine_word \<Rightarrow> machine_word) \<Rightarrow> kernel_state \<Rightarrow> kernel_state"
+where
+  "armUSGlobalPD_update f (ARMKernelState v0 v1 v2 v3 v4 v5 v6 v7) = ARMKernelState v0 v1 v2 v3 v4 v5 (f v6) v7"
 
 primrec
   armKSNextASID_update :: "(hardware_asid \<Rightarrow> hardware_asid) \<Rightarrow> kernel_state \<Rightarrow> kernel_state"
 where
-  "armKSNextASID_update f (ARMKernelState v0 v1 v2 v3 v4 v5 v6 v7) = ARMKernelState v0 v1 v2 (f v3) v4 v5 v6 v7"
+  "armKSNextASID_update f (ARMKernelState v0 v1 v2 v3 v4 v5 v6 v7) = ARMKernelState v0 v1 (f v2) v3 v4 v5 v6 v7"
 
 primrec
   armKSASIDMap_update :: "((asid \<Rightarrow> ((hardware_asid * machine_word) option)) \<Rightarrow> (asid \<Rightarrow> ((hardware_asid * machine_word) option))) \<Rightarrow> kernel_state \<Rightarrow> kernel_state"
 where
-  "armKSASIDMap_update f (ARMKernelState v0 v1 v2 v3 v4 v5 v6 v7) = ARMKernelState v0 v1 v2 v3 (f v4) v5 v6 v7"
+  "armKSASIDMap_update f (ARMKernelState v0 v1 v2 v3 v4 v5 v6 v7) = ARMKernelState v0 v1 v2 (f v3) v4 v5 v6 v7"
 
 abbreviation (input)
-  ARMKernelState_trans :: "(machine_word) \<Rightarrow> (asid \<Rightarrow> ((machine_word) option)) \<Rightarrow> (hardware_asid \<Rightarrow> (asid option)) \<Rightarrow> (hardware_asid) \<Rightarrow> (asid \<Rightarrow> ((hardware_asid * machine_word) option)) \<Rightarrow> (machine_word) \<Rightarrow> ((machine_word * bool) option) \<Rightarrow> (nat) \<Rightarrow> (machine_word \<Rightarrow> arm_vspace_region_use) \<Rightarrow> kernel_state" ("ARMKernelState'_ \<lparr> armKSGlobalsFrame= _, armKSASIDTable= _, armKSHWASIDTable= _, armKSNextASID= _, armKSASIDMap= _, armUSGlobalPT= _, armHSCurVCPU= _, armKSGICVCPUNumListRegs= _, armKSKernelVSpace= _ \<rparr>")
+  ARMKernelState_trans :: "(asid \<Rightarrow> ((machine_word) option)) \<Rightarrow> (hardware_asid \<Rightarrow> (asid option)) \<Rightarrow> (hardware_asid) \<Rightarrow> (asid \<Rightarrow> ((hardware_asid * machine_word) option)) \<Rightarrow> ((machine_word * bool) option) \<Rightarrow> (nat) \<Rightarrow> (machine_word) \<Rightarrow> (machine_word \<Rightarrow> arm_vspace_region_use) \<Rightarrow> kernel_state" ("ARMKernelState'_ \<lparr> armKSASIDTable= _, armKSHWASIDTable= _, armKSNextASID= _, armKSASIDMap= _, armHSCurVCPU= _, armKSGICVCPUNumListRegs= _, armUSGlobalPD= _, armKSKernelVSpace= _ \<rparr>")
 where
-  "ARMKernelState_ \<lparr> armKSGlobalsFrame= v0, armKSASIDTable= v1, armKSHWASIDTable= v2, armKSNextASID= v3, armKSASIDMap= v4, armUSGlobalPT= v5, armHSCurVCPU= v6, armKSGICVCPUNumListRegs= v7, armKSKernelVSpace= v8 \<rparr> == ARMKernelState v0 v1 v2 v3 v4 v5 v6 v7 v8"
+  "ARMKernelState_ \<lparr> armKSASIDTable= v0, armKSHWASIDTable= v1, armKSNextASID= v2, armKSASIDMap= v3, armHSCurVCPU= v4, armKSGICVCPUNumListRegs= v5, armUSGlobalPD= v6, armKSKernelVSpace= v7 \<rparr> == ARMKernelState v0 v1 v2 v3 v4 v5 v6 v7"
 
-lemma armKSGlobalsFrame_armKSGlobalsFrame_update [simp]:
-  "armKSGlobalsFrame (armKSGlobalsFrame_update f v) = f (armKSGlobalsFrame v)"
-  by (cases v) simp
-
-lemma armKSGlobalsFrame_armKSASIDTable_update [simp]:
-  "armKSGlobalsFrame (armKSASIDTable_update f v) = armKSGlobalsFrame v"
-  by (cases v) simp
-
-lemma armKSGlobalsFrame_armKSGlobalPD_update [simp]:
-  "armKSGlobalsFrame (armKSGlobalPD_update f v) = armKSGlobalsFrame v"
-  by (cases v) simp
-
-lemma armKSGlobalsFrame_armKSHWASIDTable_update [simp]:
-  "armKSGlobalsFrame (armKSHWASIDTable_update f v) = armKSGlobalsFrame v"
-  by (cases v) simp
-
-lemma armKSGlobalsFrame_armKSKernelVSpace_update [simp]:
-  "armKSGlobalsFrame (armKSKernelVSpace_update f v) = armKSGlobalsFrame v"
-  by (cases v) simp
-
-lemma armKSGlobalsFrame_armHSCurVCPU_update [simp]:
-  "armKSGlobalsFrame (armHSCurVCPU_update f v) = armKSGlobalsFrame v"
-  by (cases v) simp
-
-lemma armKSGlobalsFrame_armKSNextASID_update [simp]:
-  "armKSGlobalsFrame (armKSNextASID_update f v) = armKSGlobalsFrame v"
-  by (cases v) simp
-
-lemma armKSGlobalsFrame_armKSASIDMap_update [simp]:
-  "armKSGlobalsFrame (armKSASIDMap_update f v) = armKSGlobalsFrame v"
-  by (cases v) simp
-
-lemma armKSASIDTable_armKSGlobalsFrame_update [simp]:
-  "armKSASIDTable (armKSGlobalsFrame_update f v) = armKSASIDTable v"
-  by (cases v) simp
-
-lemma armKSASIDTable_armKSASIDTable_update [simp]:
-  "armKSASIDTable (armKSASIDTable_update f v) = f (armKSASIDTable v)"
-  by (cases v) simp
-
-lemma armKSASIDTable_armKSGlobalPD_update [simp]:
-  "armKSASIDTable (armKSGlobalPD_update f v) = armKSASIDTable v"
-  by (cases v) simp
-
-lemma armKSASIDTable_armKSHWASIDTable_update [simp]:
-  "armKSASIDTable (armKSHWASIDTable_update f v) = armKSASIDTable v"
-  by (cases v) simp
-
-lemma armKSASIDTable_armKSKernelVSpace_update [simp]:
-  "armKSASIDTable (armKSKernelVSpace_update f v) = armKSASIDTable v"
-  by (cases v) simp
-
-lemma armKSASIDTable_armHSCurVCPU_update [simp]:
-  "armKSASIDTable (armHSCurVCPU_update f v) = armKSASIDTable v"
-  by (cases v) simp
-
-lemma armKSASIDTable_armKSNextASID_update [simp]:
-  "armKSASIDTable (armKSNextASID_update f v) = armKSASIDTable v"
-  by (cases v) simp
-
-lemma armKSASIDTable_armKSASIDMap_update [simp]:
-  "armKSASIDTable (armKSASIDMap_update f v) = armKSASIDTable v"
-  by (cases v) simp
-
-lemma armKSGlobalPD_armKSGlobalsFrame_update [simp]:
-  "armKSGlobalPD (armKSGlobalsFrame_update f v) = armKSGlobalPD v"
-  by (cases v) simp
-
-lemma armUSGlobalPT_armHSCurVCPU_update [simp]:
-  "armUSGlobalPT (armHSCurVCPU_update f v) = armUSGlobalPT v"
-  by (cases v) simp
-
-lemma armKSGlobalPD_armKSGlobalPD_update [simp]:
-  "armKSGlobalPD (armKSGlobalPD_update f v) = f (armKSGlobalPD v)"
-  by (cases v) simp
-
-lemma armKSGlobalPD_armKSHWASIDTable_update [simp]:
-  "armKSGlobalPD (armKSHWASIDTable_update f v) = armKSGlobalPD v"
-  by (cases v) simp
-
-lemma armKSGlobalPD_armKSKernelVSpace_update [simp]:
-  "armKSGlobalPD (armKSKernelVSpace_update f v) = armKSGlobalPD v"
-  by (cases v) simp
-
-lemma armKSGlobalPD_armKSGlobalPTs_update [simp]:
-  "armKSGlobalPD (armKSGlobalPTs_update f v) = armKSGlobalPD v"
-  by (cases v) simp
-
-lemma armKSGlobalPD_armKSNextASID_update [simp]:
-  "armKSGlobalPD (armKSNextASID_update f v) = armKSGlobalPD v"
-  by (cases v) simp
-
-lemma armKSGICVCPUNumListRegs_armKSGICVCPUNumListRegs_update [simp]:
-  "armKSGICVCPUNumListRegs (armKSGICVCPUNumListRegs_update f v) = f (armKSGICVCPUNumListRegs v)"
-  by (cases v) simp
-
-lemma armKSGICVCPUNumListRegs_armKSHWASIDTable_update [simp]:
-  "armKSGICVCPUNumListRegs (armKSHWASIDTable_update f v) = armKSGICVCPUNumListRegs v"
-  by (cases v) simp
-
-lemma armKSGICVCPUNumListRegs_armKSKernelVSpace_update [simp]:
-  "armKSGICVCPUNumListRegs (armKSKernelVSpace_update f v) = armKSGICVCPUNumListRegs v"
-  by (cases v) simp
-
-lemma armKSGICVCPUNumListRegs_armHSCurVCPU_update [simp]:
-  "armKSGICVCPUNumListRegs (armHSCurVCPU_update f v) = armKSGICVCPUNumListRegs v"
-  by (cases v) simp
-
-lemma armKSGICVCPUNumListRegs_armKSNextASID_update [simp]:
-  "armKSGICVCPUNumListRegs (armKSNextASID_update f v) = armKSGICVCPUNumListRegs v"
-  by (cases v) simp
-
-lemma armKSGICVCPUNumListRegs_armKSASIDMap_update [simp]:
-  "armKSGICVCPUNumListRegs (armKSASIDMap_update f v) = armKSGICVCPUNumListRegs v"
-  by (cases v) simp
-
-lemma armKSHWASIDTable_armKSGlobalsFrame_update [simp]:
-  "armKSHWASIDTable (armKSGlobalsFrame_update f v) = armKSHWASIDTable v"
-  by (cases v) simp
-
-lemma armKSHWASIDTable_armKSASIDTable_update [simp]:
-  "armKSHWASIDTable (armKSASIDTable_update f v) = armKSHWASIDTable v"
-  by (cases v) simp
-
-lemma armKSHWASIDTable_armKSGlobalPD_update [simp]:
-  "armKSHWASIDTable (armKSGlobalPD_update f v) = armKSHWASIDTable v"
-  by (cases v) simp
-
-lemma armKSHWASIDTable_armKSHWASIDTable_update [simp]:
-  "armKSHWASIDTable (armKSHWASIDTable_update f v) = f (armKSHWASIDTable v)"
-  by (cases v) simp
-
-lemma armKSHWASIDTable_armKSKernelVSpace_update [simp]:
-  "armKSHWASIDTable (armKSKernelVSpace_update f v) = armKSHWASIDTable v"
-  by (cases v) simp
-
-lemma armKSHWASIDTable_armHSCurVCPU_update [simp]:
-  "armKSHWASIDTable (armHSCurVCPU_update f v) = armKSHWASIDTable v"
-  by (cases v) simp
-
-lemma armKSHWASIDTable_armKSNextASID_update [simp]:
-  "armKSHWASIDTable (armKSNextASID_update f v) = armKSHWASIDTable v"
-  by (cases v) simp
-
-lemma armKSHWASIDTable_armKSASIDMap_update [simp]:
-  "armKSHWASIDTable (armKSASIDMap_update f v) = armKSHWASIDTable v"
-  by (cases v) simp
-
-lemma armKSKernelVSpace_armKSGlobalsFrame_update [simp]:
-  "armKSKernelVSpace (armKSGlobalsFrame_update f v) = armKSKernelVSpace v"
+lemma armKSKernelVSpace_armKSKernelVSpace_update [simp]:
+  "armKSKernelVSpace (armKSKernelVSpace_update f v) = f (armKSKernelVSpace v)"
   by (cases v) simp
 
 lemma armKSKernelVSpace_armKSASIDTable_update [simp]:
   "armKSKernelVSpace (armKSASIDTable_update f v) = armKSKernelVSpace v"
   by (cases v) simp
 
-lemma armKSKernelVSpace_armKSGlobalPD_update [simp]:
-  "armKSKernelVSpace (armKSGlobalPD_update f v) = armKSKernelVSpace v"
+lemma armKSKernelVSpace_armKSGICVCPUNumListRegs_update [simp]:
+  "armKSKernelVSpace (armKSGICVCPUNumListRegs_update f v) = armKSKernelVSpace v"
   by (cases v) simp
 
 lemma armKSKernelVSpace_armKSHWASIDTable_update [simp]:
   "armKSKernelVSpace (armKSHWASIDTable_update f v) = armKSKernelVSpace v"
   by (cases v) simp
 
-lemma armKSKernelVSpace_armKSKernelVSpace_update [simp]:
-  "armKSKernelVSpace (armKSKernelVSpace_update f v) = f (armKSKernelVSpace v)"
-  by (cases v) simp
-
-lemma armKSKernelVSpace_armKSGlobalPTs_update [simp]:
-  "armKSKernelVSpace (armKSGlobalPTs_update f v) = armKSKernelVSpace v"
 lemma armKSKernelVSpace_armHSCurVCPU_update [simp]:
   "armKSKernelVSpace (armHSCurVCPU_update f v) = armKSKernelVSpace v"
+  by (cases v) simp
+
+lemma armKSKernelVSpace_armUSGlobalPD_update [simp]:
+  "armKSKernelVSpace (armUSGlobalPD_update f v) = armKSKernelVSpace v"
   by (cases v) simp
 
 lemma armKSKernelVSpace_armKSNextASID_update [simp]:
@@ -292,16 +144,108 @@ lemma armKSKernelVSpace_armKSASIDMap_update [simp]:
   "armKSKernelVSpace (armKSASIDMap_update f v) = armKSKernelVSpace v"
   by (cases v) simp
 
-lemma armHSCurVCPU_armKSGlobalsFrame_update [simp]:
-  "armHSCurVCPU (armKSGlobalsFrame_update f v) = armHSCurVCPU v"
+lemma armKSASIDTable_armKSKernelVSpace_update [simp]:
+  "armKSASIDTable (armKSKernelVSpace_update f v) = armKSASIDTable v"
+  by (cases v) simp
+
+lemma armKSASIDTable_armKSASIDTable_update [simp]:
+  "armKSASIDTable (armKSASIDTable_update f v) = f (armKSASIDTable v)"
+  by (cases v) simp
+
+lemma armKSASIDTable_armKSGICVCPUNumListRegs_update [simp]:
+  "armKSASIDTable (armKSGICVCPUNumListRegs_update f v) = armKSASIDTable v"
+  by (cases v) simp
+
+lemma armKSASIDTable_armKSHWASIDTable_update [simp]:
+  "armKSASIDTable (armKSHWASIDTable_update f v) = armKSASIDTable v"
+  by (cases v) simp
+
+lemma armKSASIDTable_armHSCurVCPU_update [simp]:
+  "armKSASIDTable (armHSCurVCPU_update f v) = armKSASIDTable v"
+  by (cases v) simp
+
+lemma armKSASIDTable_armUSGlobalPD_update [simp]:
+  "armKSASIDTable (armUSGlobalPD_update f v) = armKSASIDTable v"
+  by (cases v) simp
+
+lemma armKSASIDTable_armKSNextASID_update [simp]:
+  "armKSASIDTable (armKSNextASID_update f v) = armKSASIDTable v"
+  by (cases v) simp
+
+lemma armKSASIDTable_armKSASIDMap_update [simp]:
+  "armKSASIDTable (armKSASIDMap_update f v) = armKSASIDTable v"
+  by (cases v) simp
+
+lemma armKSGICVCPUNumListRegs_armKSKernelVSpace_update [simp]:
+  "armKSGICVCPUNumListRegs (armKSKernelVSpace_update f v) = armKSGICVCPUNumListRegs v"
+  by (cases v) simp
+
+lemma armKSGICVCPUNumListRegs_armKSASIDTable_update [simp]:
+  "armKSGICVCPUNumListRegs (armKSASIDTable_update f v) = armKSGICVCPUNumListRegs v"
+  by (cases v) simp
+
+lemma armKSGICVCPUNumListRegs_armKSGICVCPUNumListRegs_update [simp]:
+  "armKSGICVCPUNumListRegs (armKSGICVCPUNumListRegs_update f v) = f (armKSGICVCPUNumListRegs v)"
+  by (cases v) simp
+
+lemma armKSGICVCPUNumListRegs_armKSHWASIDTable_update [simp]:
+  "armKSGICVCPUNumListRegs (armKSHWASIDTable_update f v) = armKSGICVCPUNumListRegs v"
+  by (cases v) simp
+
+lemma armKSGICVCPUNumListRegs_armHSCurVCPU_update [simp]:
+  "armKSGICVCPUNumListRegs (armHSCurVCPU_update f v) = armKSGICVCPUNumListRegs v"
+  by (cases v) simp
+
+lemma armKSGICVCPUNumListRegs_armUSGlobalPD_update [simp]:
+  "armKSGICVCPUNumListRegs (armUSGlobalPD_update f v) = armKSGICVCPUNumListRegs v"
+  by (cases v) simp
+
+lemma armKSGICVCPUNumListRegs_armKSNextASID_update [simp]:
+  "armKSGICVCPUNumListRegs (armKSNextASID_update f v) = armKSGICVCPUNumListRegs v"
+  by (cases v) simp
+
+lemma armKSGICVCPUNumListRegs_armKSASIDMap_update [simp]:
+  "armKSGICVCPUNumListRegs (armKSASIDMap_update f v) = armKSGICVCPUNumListRegs v"
+  by (cases v) simp
+
+lemma armKSHWASIDTable_armKSKernelVSpace_update [simp]:
+  "armKSHWASIDTable (armKSKernelVSpace_update f v) = armKSHWASIDTable v"
+  by (cases v) simp
+
+lemma armKSHWASIDTable_armKSASIDTable_update [simp]:
+  "armKSHWASIDTable (armKSASIDTable_update f v) = armKSHWASIDTable v"
+  by (cases v) simp
+
+lemma armKSHWASIDTable_armKSGICVCPUNumListRegs_update [simp]:
+  "armKSHWASIDTable (armKSGICVCPUNumListRegs_update f v) = armKSHWASIDTable v"
+  by (cases v) simp
+
+lemma armKSHWASIDTable_armKSHWASIDTable_update [simp]:
+  "armKSHWASIDTable (armKSHWASIDTable_update f v) = f (armKSHWASIDTable v)"
+  by (cases v) simp
+
+lemma armKSHWASIDTable_armHSCurVCPU_update [simp]:
+  "armKSHWASIDTable (armHSCurVCPU_update f v) = armKSHWASIDTable v"
+  by (cases v) simp
+
+lemma armKSHWASIDTable_armUSGlobalPD_update [simp]:
+  "armKSHWASIDTable (armUSGlobalPD_update f v) = armKSHWASIDTable v"
+  by (cases v) simp
+
+lemma armKSHWASIDTable_armKSNextASID_update [simp]:
+  "armKSHWASIDTable (armKSNextASID_update f v) = armKSHWASIDTable v"
+  by (cases v) simp
+
+lemma armKSHWASIDTable_armKSASIDMap_update [simp]:
+  "armKSHWASIDTable (armKSASIDMap_update f v) = armKSHWASIDTable v"
+  by (cases v) simp
+
+lemma armHSCurVCPU_armKSKernelVSpace_update [simp]:
+  "armHSCurVCPU (armKSKernelVSpace_update f v) = armHSCurVCPU v"
   by (cases v) simp
 
 lemma armHSCurVCPU_armKSASIDTable_update [simp]:
   "armHSCurVCPU (armKSASIDTable_update f v) = armHSCurVCPU v"
-  by (cases v) simp
-
-lemma armHSCurVCPU_armUSGlobalPT_update [simp]:
-  "armHSCurVCPU (armUSGlobalPT_update f v) = armHSCurVCPU v"
   by (cases v) simp
 
 lemma armHSCurVCPU_armKSGICVCPUNumListRegs_update [simp]:
@@ -312,12 +256,12 @@ lemma armHSCurVCPU_armKSHWASIDTable_update [simp]:
   "armHSCurVCPU (armKSHWASIDTable_update f v) = armHSCurVCPU v"
   by (cases v) simp
 
-lemma armHSCurVCPU_armKSKernelVSpace_update [simp]:
-  "armHSCurVCPU (armKSKernelVSpace_update f v) = armHSCurVCPU v"
-  by (cases v) simp
-
 lemma armHSCurVCPU_armHSCurVCPU_update [simp]:
   "armHSCurVCPU (armHSCurVCPU_update f v) = f (armHSCurVCPU v)"
+  by (cases v) simp
+
+lemma armHSCurVCPU_armUSGlobalPD_update [simp]:
+  "armHSCurVCPU (armUSGlobalPD_update f v) = armHSCurVCPU v"
   by (cases v) simp
 
 lemma armHSCurVCPU_armKSNextASID_update [simp]:
@@ -328,28 +272,60 @@ lemma armHSCurVCPU_armKSASIDMap_update [simp]:
   "armHSCurVCPU (armKSASIDMap_update f v) = armHSCurVCPU v"
   by (cases v) simp
 
-lemma armKSNextASID_armKSGlobalsFrame_update [simp]:
-  "armKSNextASID (armKSGlobalsFrame_update f v) = armKSNextASID v"
+lemma armUSGlobalPD_armKSKernelVSpace_update [simp]:
+  "armUSGlobalPD (armKSKernelVSpace_update f v) = armUSGlobalPD v"
   by (cases v) simp
 
-lemma armKSNextASID_armKSASIDTable_update [simp]:
-  "armKSNextASID (armKSASIDTable_update f v) = armKSNextASID v"
+lemma armUSGlobalPD_armKSASIDTable_update [simp]:
+  "armUSGlobalPD (armKSASIDTable_update f v) = armUSGlobalPD v"
   by (cases v) simp
 
-lemma armKSNextASID_armKSGlobalPD_update [simp]:
-  "armKSNextASID (armKSGlobalPD_update f v) = armKSNextASID v"
+lemma armUSGlobalPD_armKSGICVCPUNumListRegs_update [simp]:
+  "armUSGlobalPD (armKSGICVCPUNumListRegs_update f v) = armUSGlobalPD v"
   by (cases v) simp
 
-lemma armKSNextASID_armKSHWASIDTable_update [simp]:
-  "armKSNextASID (armKSHWASIDTable_update f v) = armKSNextASID v"
+lemma armUSGlobalPD_armKSHWASIDTable_update [simp]:
+  "armUSGlobalPD (armKSHWASIDTable_update f v) = armUSGlobalPD v"
+  by (cases v) simp
+
+lemma armUSGlobalPD_armHSCurVCPU_update [simp]:
+  "armUSGlobalPD (armHSCurVCPU_update f v) = armUSGlobalPD v"
+  by (cases v) simp
+
+lemma armUSGlobalPD_armUSGlobalPD_update [simp]:
+  "armUSGlobalPD (armUSGlobalPD_update f v) = f (armUSGlobalPD v)"
+  by (cases v) simp
+
+lemma armUSGlobalPD_armKSNextASID_update [simp]:
+  "armUSGlobalPD (armKSNextASID_update f v) = armUSGlobalPD v"
+  by (cases v) simp
+
+lemma armUSGlobalPD_armKSASIDMap_update [simp]:
+  "armUSGlobalPD (armKSASIDMap_update f v) = armUSGlobalPD v"
   by (cases v) simp
 
 lemma armKSNextASID_armKSKernelVSpace_update [simp]:
   "armKSNextASID (armKSKernelVSpace_update f v) = armKSNextASID v"
   by (cases v) simp
 
+lemma armKSNextASID_armKSASIDTable_update [simp]:
+  "armKSNextASID (armKSASIDTable_update f v) = armKSNextASID v"
+  by (cases v) simp
+
+lemma armKSNextASID_armKSGICVCPUNumListRegs_update [simp]:
+  "armKSNextASID (armKSGICVCPUNumListRegs_update f v) = armKSNextASID v"
+  by (cases v) simp
+
+lemma armKSNextASID_armKSHWASIDTable_update [simp]:
+  "armKSNextASID (armKSHWASIDTable_update f v) = armKSNextASID v"
+  by (cases v) simp
+
 lemma armKSNextASID_armHSCurVCPU_update [simp]:
   "armKSNextASID (armHSCurVCPU_update f v) = armKSNextASID v"
+  by (cases v) simp
+
+lemma armKSNextASID_armUSGlobalPD_update [simp]:
+  "armKSNextASID (armUSGlobalPD_update f v) = armKSNextASID v"
   by (cases v) simp
 
 lemma armKSNextASID_armKSNextASID_update [simp]:
@@ -360,28 +336,28 @@ lemma armKSNextASID_armKSASIDMap_update [simp]:
   "armKSNextASID (armKSASIDMap_update f v) = armKSNextASID v"
   by (cases v) simp
 
-lemma armKSASIDMap_armKSGlobalsFrame_update [simp]:
-  "armKSASIDMap (armKSGlobalsFrame_update f v) = armKSASIDMap v"
+lemma armKSASIDMap_armKSKernelVSpace_update [simp]:
+  "armKSASIDMap (armKSKernelVSpace_update f v) = armKSASIDMap v"
   by (cases v) simp
 
 lemma armKSASIDMap_armKSASIDTable_update [simp]:
   "armKSASIDMap (armKSASIDTable_update f v) = armKSASIDMap v"
   by (cases v) simp
 
-lemma armKSASIDMap_armKSGlobalPD_update [simp]:
-  "armKSASIDMap (armKSGlobalPD_update f v) = armKSASIDMap v"
+lemma armKSASIDMap_armKSGICVCPUNumListRegs_update [simp]:
+  "armKSASIDMap (armKSGICVCPUNumListRegs_update f v) = armKSASIDMap v"
   by (cases v) simp
 
 lemma armKSASIDMap_armKSHWASIDTable_update [simp]:
   "armKSASIDMap (armKSHWASIDTable_update f v) = armKSASIDMap v"
   by (cases v) simp
 
-lemma armKSASIDMap_armKSKernelVSpace_update [simp]:
-  "armKSASIDMap (armKSKernelVSpace_update f v) = armKSASIDMap v"
-  by (cases v) simp
-
 lemma armKSASIDMap_armHSCurVCPU_update [simp]:
   "armKSASIDMap (armHSCurVCPU_update f v) = armKSASIDMap v"
+  by (cases v) simp
+
+lemma armKSASIDMap_armUSGlobalPD_update [simp]:
+  "armKSASIDMap (armUSGlobalPD_update f v) = armKSASIDMap v"
   by (cases v) simp
 
 lemma armKSASIDMap_armKSNextASID_update [simp]:
@@ -400,25 +376,19 @@ where
         alignToBits = (\<lambda>  addr b. (((addr - 1) `~shiftR~` b) + 1) `~shiftL~` b);
         globalsFrame = data_start `~alignToBits~` pageBits;
         globalsFrameTop = globalsFrame + bit pageBits;
-        globalPTs = globalsFrameTop `~alignToBits~` pageBits;
-        globalPTsTop = globalPTs + bit pageBits;
-        globalPD = globalPTsTop `~alignToBits~` pdBits;
-        globalPDTop = globalPD + bit pdBits;
-        frames = globalsFrame #
-            [globalPTs, globalPTs + bit pageBits  .e.  globalPTsTop - 1] @
-            [globalPD, globalPD + bit pageBits  .e.  globalPDTop - 1];
+        frames = error [];
         state = ARMKernelState_ \<lparr>
-            armKSGlobalsFrame= ptrFromPAddr globalsFrame,
             armKSASIDTable= funPartialArray (const Nothing) (0, (1 `~shiftL~` asidHighBits) - 1),
             armKSHWASIDTable= funArray (const Nothing),
             armKSNextASID= minBound,
             armKSASIDMap= funPartialArray (const Nothing) asidRange,
-            armUSGlobalPT= error [],
             armHSCurVCPU= Nothing,
             armKSGICVCPUNumListRegs= error [],
+            armUSGlobalPD= error [],
             armKSKernelVSpace=
                 (\<lambda> vref. if vref < mask 20 then ArmVSpaceKernelWindow
-                                            else ArmVSpaceInvalidRegion) \<rparr>
+                                            else ArmVSpaceInvalidRegion)
+            \<rparr>
     in
                                    (state, frames)"
 
