spec/design/ARM_HYP/ArchTCB_H.thy
@@ -1,3 +1,5 @@
+(* THIS FILE WAS AUTOMATICALLY GENERATED. DO NOT EDIT. *)
+(* instead, see the skeleton file ArchTCB_H.thy *)
 (*
  * Copyright 2014, General Dynamics C4 Systems
  *
@@ -11,7 +13,7 @@
 theory ArchTCB_H
 imports "../TCBDecls_H"
 begin
-context Arch begin global_naming ARM_H
+context Arch begin global_naming ARM_HYP_H
 
 definition
 decodeTransfer :: "word8 \<Rightarrow> ( syscall_error , copy_register_sets ) kernel_f"
@@ -22,6 +24,37 @@ definition
 performTransfer :: "copy_register_sets \<Rightarrow> machine_word \<Rightarrow> machine_word \<Rightarrow> unit kernel"
 where
 "performTransfer arg1 arg2 arg3 \<equiv> return ()"
+
+definition
+sanitiseRegister :: "tcb \<Rightarrow> register \<Rightarrow> machine_word \<Rightarrow> machine_word"
+where
+"sanitiseRegister tcb x1 v\<equiv> (case x1 of
+    CPSR \<Rightarrow>  
+  let
+   v' = (v && 0xf8000000) || 0x150;
+        modes = [0x10, 0x11, 0x12, 0x13, 0x17, 0x1b, 0x1f]
+  in
+  
+  if (atcbVCPUPtr (tcbArch tcb) \<noteq> Nothing \<and> ((v && 0x1f) `~elem~` modes))
+      then v
+      else v'
+  | _ \<Rightarrow>    v
+  )"
+
+
+definition
+archThreadGet :: "(arch_tcb \<Rightarrow> 'a) \<Rightarrow> machine_word \<Rightarrow> 'a kernel"
+where
+"archThreadGet f tptr\<equiv> liftM (f \<circ> tcbArch) $ getObject tptr"
+
+definition
+archThreadSet :: "(arch_tcb \<Rightarrow> arch_tcb) \<Rightarrow> machine_word \<Rightarrow> unit kernel"
+where
+"archThreadSet f tptr\<equiv> (do
+        tcb \<leftarrow> getObject tptr;
+        setObject tptr $ tcb \<lparr> tcbArch := f (tcbArch tcb) \<rparr>
+od)"
+
 
 
 end
