spec/design/ARM_HYP/RegisterSet_H.thy
@@ -1,3 +1,5 @@
+(* THIS FILE WAS AUTOMATICALLY GENERATED. DO NOT EDIT. *)
+(* instead, see the skeleton file RegisterSet_H.thy *)
 (*
  * Copyright 2014, General Dynamics C4 Systems
  *
@@ -15,7 +17,7 @@ imports
   "../../../lib/HaskellLib_H"
   "../../machine/ARM_HYP/MachineTypes"
 begin
-context Arch begin global_naming ARM_H
+context Arch begin global_naming ARM_HYP_H
 
 definition
   newContext :: "register => machine_word"
